TestsR.v
@@ -1,0 +1,91 @@
+(** * TestsR: Tests of RecordsExt.v *)
+
+(**  *)
+
+Add LoadPath "/Users/pv/Polya/Coq/pierce_software_foundations_3.2".
+Require Export SfLib.
+Require Import LibTactics.
+
+(* Require Export Stlc. *)
+Require Export Common LDef RecordsExt.
+Import P3Common LDEF Records.
+
+Module RETests.
+
+(** Some variables, for examples... *)
+
+Notation a := (Id 0).
+Notation f := (Id 1).
+Notation g := (Id 2).
+Notation l := (Id 3).
+Notation A := (TBase (Id 4)).
+Notation B := (TBase (Id 5)).
+Notation k := (Id 6).
+Notation i1 := (Id 7).
+Notation i2 := (Id 8).
+
+(** [{ i1:A }] *)
+
+Example er1 : exists (t:ty), t = TRcd [(i1, A)].
+Proof. eauto. Qed.
+
+(** [{ i1:A->B, i2:A }] *)
+Example er2 : exists (t:ty), t = 
+  TRcd [(i1, (TArrow A B)); (i2, A)].
+Proof. eauto. Qed.
+
+Definition substf_ok (sfunc:  id -> tm -> tm -> tm) :=
+  sfunc a (tvar f) (tvar a) = tvar f
+    /\ sfunc a (tvar f) (tvar g) = tvar g
+    /\ sfunc g (tvar f) (tvar a) = tvar a
+    /\ sfunc a (tvar g) (tproj (tvar a) a) = tproj (tvar g) a
+    /\ sfunc a (tvar g) (tapp (tvar f) (tvar a)) = tapp (tvar f) (tvar g)
+    /\ sfunc a  (tapp (tvar f) (tvar a)) (tproj (tvar a) a)
+        =  tproj  (tapp (tvar f) (tvar a)) a.
+
+Example subst_ok :substf_ok subst.
+Proof. unfold substf_ok. repeat split. Qed.
+
+Lemma typing_example_2 : 
+  empty |- 
+    (tapp (tabs a (TRcd [(i1, (TArrow A A)); (i2, (TArrow B B))])
+              (tproj (tvar a) i2))
+            (trcd [(i1, (tabs a A (tvar a))); (i2, (tabs a B (tvar a)))]) )
+    \in (TArrow B B).
+Proof. eauto 30 using extend_eq, eq_id. 
+       (* FIX EAUTO USAGE ABOVE *)
+  eapply T_App.
+    eapply T_Abs. eapply T_Proj.
+      eapply T_Var.  eapply eq_id.
+      reflexivity. 
+    eapply T_Rcd. eapply TR_Cons.
+      eapply T_Abs. eapply T_Var. eapply extend_eq.
+      eapply TR_Cons.
+        eapply T_Abs. eapply T_Var. eapply extend_eq.
+        eapply TR_Nil.
+Qed.
+
+(** Before starting to prove this fact (or the one above!), make sure
+    you understand what it is saying. *)
+
+Example typing_nonexample : 
+  ~ exists T,
+      (extend empty a (TRcd (cons (i2, (TArrow A A)) nil)))  |-
+               (trcd (cons (i1, (tabs a B (tvar a))) nil)) \in
+               T.
+  (* no T | a : { i2 : A->A } |- { i1 = λ a:B . a } : T *)
+Proof.
+  (* FILL IN HERE *) Admitted.
+
+Example typing_nonexample_2 : forall y,
+  ~ exists T,
+    (extend empty y A) |-
+           (tapp (tabs a (TRcd (cons (i1, A) nil))
+                     (tproj (tvar a) i1))
+                   (trcd (cons (i1, (tvar y)) (cons (i2, (tvar y)) nil))) ) \in
+           T.
+  (* forall y, ~ exists T, y : A |- (λ a : { i1 : A} . a.i1) { i1 = y; i2 = y } : T *)
+Proof.
+  (* FILL IN HERE *) Admitted.
+
+End RETests.
